Correct translation of scheduling with oracle check

src/hls/RTLPargen.v
@@ -16,12 +16,61 @@
  * along with this program.  If not, see <https://www.gnu.org/licenses/>.
  *)
 
-From compcert Require Import AST.
-From vericert Require Import RTLBlock RTLPar.
+From compcert Require Import AST Maps.
+From vericert Require Import Vericertlib RTLBlock RTLPar Scheduleoracle.
 
-Parameter schedule : RTLBlock.function -> Errors.res RTLPar.function.
+Fixpoint beq {A B : Type} (beqA : A -> B -> bool) (m1 : PTree.t A) (m2 : PTree.t B) {struct m1} : bool :=
+  match m1, m2 with
+  | PTree.Leaf, _ => PTree.bempty m2
+  | _, PTree.Leaf => PTree.bempty m1
+  | PTree.Node l1 o1 r1, PTree.Node l2 o2 r2 =>
+    match o1, o2 with
+    | None, None => true
+    | Some y1, Some y2 => beqA y1 y2
+    | _, _ => false
+    end
+    && beq beqA l1 l2 && beq beqA r1 r2
+  end.
 
-Definition transl_fundef := transf_partial_fundef schedule.
+Lemma beq_correct:
+  forall A B beqA m1 m2,
+    @beq A B beqA m1 m2 = true <->
+    (forall (x: PTree.elt),
+        match PTree.get x m1, PTree.get x m2 with
+        | None, None => True
+        | Some y1, Some y2 => beqA y1 y2 = true
+        | _, _ => False
+        end).
+Proof.
+  induction m1; intros.
+  - simpl. rewrite PTree.bempty_correct. split; intros.
+    rewrite PTree.gleaf. rewrite H. auto.
+    generalize (H x). rewrite PTree.gleaf. destruct (PTree.get x m2); tauto.
+  - destruct m2.
+    + unfold beq. rewrite PTree.bempty_correct. split; intros.
+      rewrite H. rewrite PTree.gleaf. auto.
+      generalize (H x). rewrite PTree.gleaf. destruct (PTree.get x (PTree.Node m1_1 o m1_2)); tauto.
+    + simpl. split; intros.
+      * destruct (andb_prop _ _ H). destruct (andb_prop _ _ H0).
+        rewrite IHm1_1 in H3. rewrite IHm1_2 in H1.
+        destruct x; simpl. apply H1. apply H3.
+        destruct o; destruct o0; auto || congruence.
+      * apply andb_true_intro. split. apply andb_true_intro. split.
+        generalize (H xH); simpl. destruct o; destruct o0; tauto.
+        apply IHm1_1. intros; apply (H (xO x)).
+        apply IHm1_2. intros; apply (H (xI x)).
+Qed.
+
+Parameter schedule : RTLBlock.function -> RTLPar.function.
+
+Definition transl_function (f : RTLBlock.function) : Errors.res RTLPar.function :=
+  let tf := schedule f in
+  if beq schedule_oracle f.(RTLBlock.fn_code) tf.(fn_code) then
+    Errors.OK tf
+  else
+    Errors.Error (Errors.msg "RTLPargen: Could not prove the blocks equivalent.").
+
+Definition transl_fundef := transf_partial_fundef transl_function.
 
 Definition transl_program (p : RTLBlock.program) : Errors.res RTLPar.program :=
   transform_partial_program transl_fundef p.
